[Iterative Lanczos and Orthogonal Polynomials](Iterative%20Lanczos%20and%20Orthogonal%20Polynomials.md)
[Symmetric Tridiagonal Matrices Recursive Det](Symmetric%20Tridiagonal%20Matrices%20Recursive%20Det.md)

---
### **Intro**

There is a relations between the orthogonal polynomials representing the lanczos vector $q_k$ in the krylov subspace, and the characteristic polynomial of $T_k$ during that iterations. Let $p_k(x)$ denotes the characteristic polynomial for $T_k$ generated by the Iterative Lanczos algorithm, and let $\psi_k$ denotes the $k - 1$ degree polynomial of $q_k$ represented under Krylov Subspace, then:

> $$
> \begin{aligned}
>     \psi_k(x) = \left(\prod_{i = 1}^{k-1} \beta_i\right)^{-1}(-1)^{k - 1}p_{k - 1}(x)
> \end{aligned}
> $$

As a corollary of the theorem, the characteristic polynomial of the symmetric tridiagonal matrix generated by the Lanczos iteration is also orthogonal over the same weighted discrete measure that $\psi_j$ is in. 

---
### **Proof**
Suppose that the recursion for the cahracterstic polynomial for $T_k$ is true, and inductively we assume that formulas: 

$$
\begin{aligned}
    & 
    \psi_j(x) = \left(\prod_{i = 1}^{j-1} \beta_i\right)^{-1}
    (-1)^{j - 1}p_{j - 1}(x)
    \quad \forall\; 1 \le j \le k
    \\
    & 
    \begin{cases}
        \beta_j \psi_{j + 1} = 
        (x - \alpha_j)\psi_j - \beta_{j - 1}\psi_{j -1}    
        & \forall j \ge 2
        \\
        \psi_1 = 1
        \\
        \psi_0 = 0
    \end{cases}
    \\
    &
    \begin{cases}
        p_j(x) = (\alpha_j - x)p_{j - 1}(x) - \beta_{j - 1}^2p_{j - 1}(x)    
        &
        \forall j \ge 1
        \\
        p_0(x) = 1 
        \\
        p_{-1}(x) = 0
    \end{cases}
\end{aligned}
$$

Firstly, the base case matches by definition. Assume the recursion for j th characterstic polynomial and the orthogonal polynomials are true, we inductively prove the relations between them holds up for $j = k + 1$. Let's consider: 

$$
\begin{aligned}
    \beta_j\psi_{j + 1} &=
    x \psi_j - \alpha_j \psi + \beta_{j - 1}\psi_{j - 1}
    \\
    &= (x - \alpha_j)\psi_j + \beta_{j - 1}\psi_{j - 1}
    \\
    &= (x - \alpha_j)\left(
        \prod_{i = 1}^{j - 1}\beta_i
    \right)^{-1}(-1)^{j + 1}p_{j - 1}
    + 
    \beta_{j - 1}\left(
        \prod_{i = 1}^{j - 2}\beta_i
    \right)^{-1}(-1)^{j}p_{j - 2}
    \\
    &= 
    \left(
        \prod_{i = 1}^{j - 2}\beta_i
    \right)^{-1}
    \left(
        (x - \alpha_j)\beta_{j - 1}^{-1}(-1)^{j + 1}p_{j + 1}
        + 
        \beta_{j - 1}(-1)^jp_{j -2}
    \right)
    \\
    &= 
    \left(
        \prod_{i = 1}^{j - 2}\beta_i
    \right)^{-1}
    (-1)^{j}
    \left(
        (\alpha_j - x)\beta_{j - 1}^{-1}p_{j + 1}
        + 
        \beta_{j - 1}p_{j -2}
    \right)
    \\
    &=
    \left(
        \prod_{i = 1}^{j - 2}\beta_i
    \right)^{-1}
    (-1)^{j}\beta_{j - 1}^{-1}
    \underbrace{\left(
        (\alpha_j - x)p_{j + 1}
        + 
        \beta_{j - 1}^2p_{j -2}
    \right)}_{=p_j(x)}
    \\
    &= 
    \left(
        \prod_{i = 1}^{j - 1}\beta_i
    \right)^{-1}(-1)^{j + 2}p_j(x)
    \\
    \implies  \beta_j\psi_{j + 1} &= \left(
        \prod_{i = 1}^{j - 1}\beta_i
    \right)^{-1}(-1)^{j + 2}p_j(x)
\end{aligned}
$$
The recursion holds up. 

